

Q4.1.

Proof: Suppose,  $0 \leq s \leq t \leq T$ , for the purpose of proving  $I(t)$  is a martingale is to prove  $E[I(t)|F_s] = I(s)$

Case 1.  $t$  and  $s$  are in the same subinterval.  $[t_k, t_{k+1}]$

$$I(s) = \sum_{j=0}^{k-1} \Delta(t_j) [M(t_{j+1}) - M(t_j)] + \Delta(t_k) [M(t_s) - M(t_k)] \quad (1)$$

$$I(t) = \sum_{j=0}^{k-1} \Delta(t_j) [M(t_{j+1}) - M(t_j)] + \Delta(t_k) [M(t) - M(t_k)] \quad (2)$$

$$\text{for } E[I(t)|F_s] = E[I(t) - I(s) + I(s)|F_s] = E[I(t) - I(s)|F_s] + E[I(s)|F_s]$$

$(I(t) - I(s) \text{ is independent of } F_s, I(s) \text{ is } F_s\text{-measurable})$

$$= \Delta(t_k) E[M(t) - M(s)] + I(s) \quad (\Delta(t_k) \text{ is } F_s\text{-measurable})$$

$$= I(s) \quad (E[M(t) - M(s)] = 0)$$

Case 2.  $t$  and  $s$  are in the different subinterval  $[t_k, t_{k+1}], [t_l, t_{l+1}]$   $k < l$

$$I(t) = \underbrace{\sum_{j=0}^{k-1} \Delta(t_j) [M(t_{j+1}) - M(t_j)]}_{(1)=V_1} + \underbrace{\Delta(t_k) [M(t_{k+1}) - M(t_k)]}_{(2)=V_2} + \underbrace{\sum_{j=k+1}^{l-1} \Delta(t_j) [M(t_{j+1}) - M(t_j)]}_{(3)=V_3} + \underbrace{\Delta(t_l) [M(t) - M(t_l)]}_{(4)=V_4}$$

$$E[I(t)|F_s] = E[V_1|F_s] + E[V_2|F_s] + E[V_3|F_s] + E[V_4|F_s]$$

for (1). (1) is  $F_s$ -measurable.  $\Rightarrow E[V_1|F_s] = V_1$

$$\text{for (3), (4) are independent of } F_s. \quad E[V_3|F_s] = \sum_{j=k+1}^{l-1} E[E[\Delta(t_j) (M(t_{j+1}) - M(t_j)) | F_{t_j}]] | F_s]$$

$i > s$ .

$$= \sum_{j=k+1}^{l-1} E[\Delta(t_j) E[M(t_{j+1}) - M(t_j) | F_s]] = \sum_{j=k+1}^{l-1} E[\Delta(t_j) \cdot 0 | F_s] = 0.$$

$$E[V_4|F_s] = E[\Delta(t_l) (M(t) - M(t_l)) | F_{t_l} | F_s] = E[\Delta(t_l) \cdot 0 | F_s] = 0.$$

$$\text{for (2). } E[\Delta(t_k) (M(t_{k+1}) - M(s) + M(s) - M(t_k)) | F_s] = \Delta(t_k) (E[M(t_{k+1}) - M(s) | F_s] + M(s) - M(t_k)) = \Delta(t_k) (M(s) - M(t_k))$$

$$\therefore (1) + (2) + (3) + (4) = \sum_{j=0}^{k-1} \Delta(t_j) [M(t_{j+1}) - M(t_j)] + \Delta(t_k) (M(s) - M(t_k)) = I(s)$$

(concluded)

Q4.3.  
(i).  $s, t$  is the point in the subinterval  $[s, t)$

(2)

$$\text{So, } I(t) - I(s) = \Delta(s) (W(t) - W(s)) \\ = W(s) (W(t) - W(s))$$

$W(s)$  is  $\mathcal{F}_s$ -measurable, not independent of  $\mathcal{F}_s$   
(ii). use hint to prove.

$$\text{let } X = \frac{E[(I(t) - I(s))^4]}{D^2[I(t) - I(s)]}$$

$\therefore I(s)$  is in the same interval.

$$\therefore E[I(t) - I(s)] = E[W(s)(W(t) - W(s))] \\ = E[W(s)] \cdot E[W(t) - W(s)]$$

$W(s)$  is independent of  $W(t) - W(s)$

$$= \frac{E[W(s)]^4 \cdot E[W(t) - W(s)]^4}{D^2[I(t) - I(s)]}$$

$$E[W(s)] \sim N(0, s), \quad W(t) - W(s) \sim N(0, t-s), \quad E[W(s)]^4 = 3s, \quad E[W(t) - W(s)]^4 = 3(t-s)$$

$$D^2[I(t) - I(s)] = (E[I(t) - I(s)]^2 + E^2(I(t) - I(s)))^2 = E^2(I(t) - I(s))^2 = (E[W(s)]^2 \cdot E[W(t) - W(s)]^2)^2 \\ = (D(W(s)) \cdot D(W(t) - W(s)))^2 \\ = s^2 \cdot (t-s)^2$$

$$X = \frac{9s(t-s)}{s^2(t-s)^2} = \frac{9}{s(t-s)} \neq 3$$

$\therefore I(t) - I(s)$  is not 'Normally Distribution'.

$$(iii) \quad E[I(t) - I(s)] = E[I(t) | \mathcal{F}_s] - E[I(s) | \mathcal{F}_s]$$

$$= E(W(s)(W(t) - W(s)) | \mathcal{F}_s) + E[W(s) | \mathcal{F}_s]$$

$$= W(s) \cdot E[W(t) - W(s)] + I(s)$$

$$= 0 + I(s) = I(s)$$

$$\text{besides, } I(s) = W(s) \cdot (W(s) - W(s)) = 0.$$

(iv) defined by Itô Integral.

$$I(t) = 0 + W(s)(W(t) - W(s))$$

right.  $I^2(s) = [W(s)(W(s) - W(s))]^2 = 0$

$$\int_0^s \Delta^2 u du = \int_0^s 0 du = 0$$

$$I^2(s) - \int_0^s \Delta^2 u du = 0$$

$$\text{left, } E[I^2(t) | \mathcal{F}_s] = E[W(s)^2 \cdot (W(t) - W(s))^2 | \mathcal{F}_s] = W(s)^2 \cdot (t-s)$$

$$E\left[\int_0^t \Delta^2 u du | \mathcal{F}_s\right] = \int_0^s \Delta^2 u du + E\left[\int_s^t \Delta^2 u du | \mathcal{F}_s\right]$$

$$= 0 + \int_s^t W(s)^2 du = W(s)^2 (t-s)$$

$$\therefore E[I^2(t) - \int_0^t \Delta^2 u du | \mathcal{F}_s] = 0$$

in a sum

$$E[I^2(t) - \int_0^t \Delta^2 u du | \mathcal{F}_s] = I^2(s) - \int_0^s \Delta^2 u du$$

Q4.5

(3)

~~(i)  $S(t) = S_0 e^{X(t)} = S_0 e^{\int_0^t G(s) dW(s) + \int_0^t (2(s) - \frac{1}{2} G^2(s)) ds}$~~

~~$\log_e S(t) = \log_e S_0 + \int_0^t G(s) dW(s) + \int_0^t (2(s) - \frac{1}{2} G^2(s)) ds$~~

$\log S(t)$  means  $\log_e S(t)$ .  $\ln S(t)$  is an

~~$\frac{dS(t)}{S(t)}$~~   $f(S(t)) = \ln S(t)$

$$df(S(t)) = \underbrace{f'(S(t)) dS(t)}_{(1)} + \underbrace{\frac{1}{2} f''(S(t)) dS(t) dS(t)}_{(2)} + \underbrace{\text{higher order term}}_{(3)}$$

any term in (3):  $dS(t) \cdot dS(t) = 2^2(t) S^2(t) dt \cdot dt + 2(t) \cdot G(t) \cdot S(t) dW(t) dt + G^2(t) \cdot S^2(t) dW(t) dW(t)$   
 $= 0 + 0 + G^2(t) \cdot S^2(t) dt = G^2(t) S^2(t) dt$

$\therefore$  (3) must either contain  $dW(t) \cdot dt = 0$  or  $dt \cdot dt = 0$

$$\therefore (3) = 0$$

$$(2) + (1) \frac{dS(t)}{S(t)} = 2(t) \cdot dt + G(t) \cdot dW(t) + \frac{1}{2} G^2(t) \cdot S^2(t) dt = G(t) dW(t) + (2(t) - \frac{1}{2} G^2(t)) dt$$

in a sum

~~$\frac{dS(t)}{S(t)}$~~   $d(\ln S(t)) = G(t) dW(t) + (2(t) - \frac{1}{2} G^2(t)) dt$

(ii). integrate  $d(\ln S(t))$ ,  $\ln S(t) \Big|_0^t = \int_0^t G(u) dW(u) + (2(u) - \frac{1}{2} G^2(u)) du$

~~$\ln S(t) = \int_0^t \frac{1}{S(u)} dS(u) = \int_0^t G(u) dW(u) + \int_0^t (2(u) - \frac{1}{2} G^2(u)) du$~~

$$\ln S(t) = \ln S_0 + \int_0^t G(u) dW(u) + \int_0^t (2(u) - \frac{1}{2} G^2(u)) du$$

$$S(t) = S_0 \cdot e^{\int_0^t G(u) dW(u) + \int_0^t (2(u) - \frac{1}{2} G^2(u)) du}$$

get function  
(4.4.26)

Q 4.7.  $f(x) = x^4$ 

$$(i) dW_t^4 = f'(W_t) dW_t + \frac{1}{2} f''(W_t) dt$$

$$= 4W_t^3 dW_t + 6W_t^2 dt$$

$$W_t^4|_0^T = \int_0^T 4W_u^3 dW_u + \int_0^T 6W_u^2 du$$

$$W^4(T) = W^4(0) + \int_0^T 4W_u^3 dW_u + \int_0^T 6W_u^2 du$$

$$= 4 \int_0^T W_u^3 dW_u + 6 \int_0^T W_u^2 du$$

$$(ii) E(W^4(T)) = 4 E\left[\int_0^T W_u^3 dW_u\right] + 6 E\left[\int_0^T W_u^2 du\right]$$

$$= 4 \cdot 0 + 6 \int_0^T E[W_u^2] du$$

$$= 6 \cdot \int_0^T u du = 3T^2$$

Itô Integral is a martingale.

$\int_0^T W_u^3 dW_u$  is an Itô Integral.  
whose expectation is 0.

(iii) similar to i.

$$dW_t^6 = 6W_t^5 dt + 15W_t^4 dt$$

$$W^6(T) = 6 \int_0^T W_u^5 du + 15 \int_0^T W_u^4 du$$

similar to ii

$$E W^6(T) = 0 + 15 \int_0^T E[W_u^4] du = 15 \cdot T^3$$

Q.4.8.

$$f(t, R_t) = e^{\beta t} \cdot R_t$$

(5)

$$(i). d(e^{\beta t} R_t) = \beta \cdot e^{\beta t} R_t dt + e^{\beta t} dR_t \quad \# R_t = \beta \cdot e^{\beta t} R_t dt + e^{\beta t} [\alpha - \beta R_t] dt + \sigma dW_t$$

$$f_t(t, R_t) = e^{\beta t} R_t$$

$$f_{R_t}(t, R_t) = e^{\beta t}$$

$$f_{RR_t}(t, R_t) = 0$$

$$\text{thus } d(e^{\beta t} R_t) = e^{\beta t} (\alpha dt + \sigma dW_t)$$

$$(ii). e^{\beta t} R_t \Big|_0^T = \int_0^T e^{\beta t} (\alpha dt) + e^{\beta t} \cdot \sigma dW_t$$

$$e^{\beta T} R(T) - R(0) = \int_0^T \frac{\alpha}{\beta} (e^{\beta T} - 1) + \sigma \int_0^T e^{\beta t} dW_t$$

$$R(T) = \frac{\alpha}{\beta} (1 - e^{-\beta T}) + \sigma \int_0^T e^{\beta(t-T)} dW_t + R_0$$

Q. addition

$$a). X_t = f(t, W_t) = e^{t W_t}$$

$$f_t = W_t e^{t W_t}$$

~~$$dX_t = \frac{1}{2} W_t^2 e^{t W_t} dt + \int t \cdot e^{t W_t} dW_t + \int t^2 \cdot e^{t W_t} dt$$~~

$$f_{XX} = t e^{t W_t}$$

$$dX_t = W_t e^{t W_t} dt + t \cdot e^{t W_t} dW_t + \frac{1}{2} t^2 e^{t W_t} dt$$

$$f_{XX} = t^2 e^{t W_t}$$

$$b). \text{ when } X_t = e^{rt} f(W_t) \text{ let } g(t, W_t) = X_t$$

$$g_t(t, W_t) = r e^{rt} f(W_t) \neq e^{rt} f'$$

$$g_X(t, W_t) = e^{rt} f'(W_t)$$

$$g_{XX}(t, W_t) = e^{rt} f''(W_t) = \lambda e^{rt} f(W_t)$$

$$dX_t = r e^{rt} f(W_t) dt + e^{rt} f'(W_t) dW_t + \frac{1}{2} \lambda e^{rt} f(W_t) dt$$

$$X_t = X_0 + \int_0^t r e^{ru} f(W_u) du + \int_0^t e^{ru} f'(W_u) dW_u + \int_0^t \frac{1}{2} \lambda e^{ru} f(W_u) du$$

$$X_t = 1 + \int_0^t (r + \frac{\lambda}{2}) e^{ru} f(W_u) du + \int_0^t e^{ru} f'(W_u) dW_u$$

$$E[X_t] = 1 + E\left[\int_0^t (r + \frac{\lambda}{2}) e^{ru} f(W_u) du\right]$$

$$E\left[\frac{X_t}{e^{rt}}\right] = e^{-rt} + e^{rt} E\left[\int_0^t (r + \frac{\lambda}{2}) e^{ru} f(W_u) du\right]$$

$$\text{when } r + \frac{\lambda}{2} = 0, \quad -r = \frac{\lambda}{2}$$

$$E[f(W_t)] = e^{\frac{\lambda}{2} t} + a$$

$$= e^{\frac{\lambda}{2} t}$$

Recommend. 如何理解非随机过程

⑥

Q4.2

(i): for  $I(t) - I(s)$ , because  $\Delta(t)$  is a nonrandom simple process, we know  $\Delta(t_k)$  at time  $t_k$ , when  $t_k > t_i$ .

so we can divide the interval  $[t_s, t_{s+1})$  into  $[t_s, s)$  and  $[s, t_{s+1})$ , suppose  $s \in [t_k, t_{k+1})$  thus,  $I(s)$  also equals to.

$$I(s) = \lim_{i \rightarrow 0} \sum_{j=0}^{k-1} \Delta(t_{j+1}) [W(t_{j+1}) - W(t_j)] + \Delta(t_{k+1}) [W(s) - W(t_k)],$$

We use the new definition of  $I(s)$ .

$$I(t) - I(s) = \lim_{i \rightarrow 0} \left( \sum_{j=s}^{t-1} \Delta(t_{j+1}) [W(t_{j+1}) - W(t_j)] + \Delta(t_{k+1}) [W(t) - W(t_k)] \right)$$

- ① in every part  $\lim_{i \rightarrow 0} (\Delta(t_{j+1}) [W(t_{j+1}) - W(t_j)])$  (when  $j > s$ ) is independent of  $F_s$ .
- ② in the part  $\lim_{i \rightarrow 0} \Delta(t_{k+1}) [W(t_{k+1}) - W(s)]$ ,  $\Delta(t_{k+1})$  and  $W(t_{k+1}) - W(s)$  are both independent of  $F_s$ .

In a sum,  $I(t) - I(s)$  is independent of  $F_s$ .

(ii). proved by (i).  $I(t) - I(s)$  is independent of  $F_s$ .

So, for every subinterval  $[t_k, t_i]$ ,  $t_k, t_i$  is the partition point and  $t_k < t_i$ .  $I(t_k) - I(t_k)$  is independent of  $F(t_k) \Rightarrow D(X+Y) = D(X) + D(Y)$

thus,  $I(t) - I(s) = \sum_{i=0}^{n-1} (I(x_{i+1}) - I(x_i))$  is a partition between  $s$  and  $t$ ,  $\{x_0=s, x_1, x_2, \dots, x_n=t\}$

$$I(t) - I(s) = \sum_{i=0}^{n-1} (I(x_{i+1}) - I(x_i))$$

for each  $I(x_{i+1}) - I(x_i) = \Delta(x_i) (W(x_{i+1}) - W(x_i)) \sim N(0, \Delta(x_i)^2 (x_{i+1} - x_i))$   
(正态分布相加?)

$$I(t) - I(s) \sim N(0, \sum_{i=0}^{n-1} \Delta(x_i)^2 (x_{i+1} - x_i))$$

$\Delta(x)$  is a constant  $\therefore \Delta(x_i)^2$  is a constant.

$$\Delta(x_i)^2 (x_{i+1} - x_i) = \int_{x_i}^{x_{i+1}} \Delta^2(u) du$$

$$\therefore I(t) - I(s) \sim N(0, \int_s^t \Delta^2(u) du)$$

Q. 4.6.

$S(t)$  is a geometric Brownian Motion

$$dS(t) = \alpha(t) S(t) dt + \sigma(t) S(t) dW(t)$$

$$\therefore f(x) = x^p, \quad f'(x) = p x^{p-1}, \quad f''(x) = p(p-1) x^{p-2}$$

$$df(S) = p \cdot S^{p-1} \cdot dS(t) + \frac{p(p-1)}{2} \frac{dS(t)^2}{dt} dt$$

$$= p \cdot S^{p-1} (\alpha S dt + \sigma S dW) + \frac{p(p-1)}{2} \cdot \sigma^2 S^2 dt$$

$$= p \cdot S^p (\alpha dt + \sigma dW) + \frac{p(p-1)}{2} \sigma^2 S^2 dt$$

$$= (p \alpha \cdot S^p + \frac{p(p-1)}{2} \sigma^2 S^2) dt + p \cdot \sigma S^p \cdot dW(t)$$

~~$$dS(t) \cdot dS(t) = (\alpha S dt + \sigma S dW) dt + \sigma^2 S^2 dt + \sigma^2 S^2 dW dt$$~~

~~$$= \alpha S^2 dt + \sigma^2 S^2 dt + \sigma^2 S^2 dW dt$$~~

$$dS(t) \cdot dS(t) = 0 + 0 + 0 + \sigma^2 S^2 dt = \sigma^2 S^2 dt$$